Promises.Examples: an (almost) interesting example

share/steel/examples/pulse/parix/Promises.Examples.fst
@@ -1,23 +1,15 @@
 module Promises.Examples
 
 open Pulse.Lib.Pervasives
-open Promises
+open Promises.Temp
 
 #set-options "--ext pulse:guard_policy=SMTSync"
-(* Assuming invariants *)
+#set-options "--print_implicits"
 
-[@@erasable]
-assume val inv : vprop -> Type0
+(* Assuming invariants *)
 
 // should be ghost
 assume val mk_inv : p:vprop -> stt (inv p) p (fun _ -> emp)
-
-assume val with_inv
-  (#a:Type0) (#pre : vprop) (#post : (a -> vprop))
-  (#p:vprop)
-  (i:inv p)
-  ($f : unit -> stt_ghost a emp_inames (p ** pre) (fun r -> p ** post r))
-  : stt_ghost a emp_inames pre post
 
 assume val admit_ghost
   (#a:Type0) (#pre : vprop) (#post : (a -> vprop))
@@ -26,49 +18,42 @@ assume val admit_ghost
 
 type abc = | A | B | C
 
-
 let invp (b:ref abc) (y:ref int) =
-  exists_ (fun (bb:abc) -> pts_to b #(half_perm full_perm) bb ** (if bb = B then pts_to y 42 else emp))
+  exists_ (fun (bb:abc) -> pts_to b #one_half bb ** (if bb = B then pts_to y 42 else emp))
 
 ```pulse
 fn test_aux (b : ref abc) (y : ref int)
-  requires pts_to b #(half_perm full_perm) B ** invp b y
-  ensures pts_to b #(half_perm full_perm) C ** pts_to y 42 ** invp b y
+  requires pts_to b #one_half B ** invp b y
+  ensures pts_to b #one_half C ** pts_to y 42 ** invp b y
 {
   unfold invp b y;
   with bb.
-    assert (pts_to b #(half_perm full_perm) bb ** `@(if bb = B then pts_to y 42 else emp));
+    assert (pts_to b #one_half bb ** `@(if bb = B then pts_to y 42 else emp));
 
-  assert (pts_to b #(half_perm full_perm) B);
-  assert (pts_to b #(half_perm full_perm) bb);
+  assert (pts_to b #one_half B);
+  assert (pts_to b #one_half bb);
 
   // Automate?
   pts_to_injective_eq #abc
-        #(half_perm full_perm) #(half_perm full_perm)
+        #one_half #one_half
         #B #bb
         b;
 
-  // Automate?
-  rewrite (pts_to b #(half_perm full_perm) bb)
-       as (pts_to b #(half_perm full_perm) B);
+  assert (pts_to b #one_half (reveal (hide B)) ** pts_to b #one_half (reveal (hide B)));
 
   gather2 #abc #emp_inames b;
 
-  // Should automate
-  rewrite (pts_to b #(sum_perm (half_perm full_perm) (half_perm full_perm)) true)
-       as (pts_to b true);
+  b := C; // The only non-ghost step
 
-  assert (pts_to b #full_perm true);
-
-  b := false;
-
-  share b;
+  share2 #_ #emp_inames b;
 
   rewrite emp
        as (`@(if false then pts_to y 42 else emp));
 
-  intro_exists (fun (bb:bool) -> pts_to b #(half_perm full_perm) bb ** (if bb then pts_to y 42 else emp))
-    false;
+  intro_exists (fun (bb:abc) -> pts_to b #one_half bb ** (if bb = B then pts_to y 42 else emp))
+    C;
+
+  assert (pts_to y 42);
 
   fold invp b y;
 
@@ -76,39 +61,130 @@ fn test_aux (b : ref abc) (y : ref int)
 }
 ```
 
+```pulse
+fn test_aux_with_inv (b : ref abc) (y : ref int) (i : inv (invp b y))
+  requires pts_to b #one_half B
+  ensures pts_to b #one_half C ** pts_to y 42
+{
+   with_invariants i {
+     test_aux b y
+   }
+}
+```
+
+let pts_to_b_or_c (b : ref abc) =
+  exists_ (fun (v:abc) -> pts_to b #one_half v ** pure (B? v \/ C? v))
+
+```pulse
+fn test_aux_with_inv2 (b : ref abc) (y : ref int) (i : inv (invp b y))
+  requires pts_to_b_or_c b ** emp
+  ensures pts_to_b_or_c b ** pts_to y 42
+{
+   (* This would be a ghost read.. *)
+   unfold (pts_to_b_or_c b);
+   let v = !b;
+   match v {
+      B -> {
+        with_invariants i ensures pts_to b #one_half C ** pts_to y 42
+        {
+          test_aux b y
+        };
+        assert (exists_ (fun (v:abc) -> pts_to b #one_half v ** pure (B? v \/ C? v)));
+        fold pts_to_b_or_c b;
+        ()
+      }
+      C -> {
+        // Ouch... I thought this was ok, but I don't see how to prove
+        // this case. Maybe the way to go is store some permission
+        // to B in the promise itself.
+        admit ()
+      }
+   }
+}
+```
+
+#set-options "--split_queries always"
+
 
 (* Promising and redeeming in a single func *)
 ```pulse
-fn test (b : ref bool) (y : ref int)
-  requires pts_to b false ** pts_to y yy
+fn test (b : ref abc) (y : ref int)
+  requires pts_to b A ** pts_to y yy
   returns x:int
-  ensures promise (pts_to b true) (pts_to y 42)
+  ensures pts_to y 42
 {
-  assert (pts_to b false);
-  share b;
-  assert (pts_to b #(half_perm full_perm) false);
-  assert (pts_to b #(half_perm full_perm) false ** emp);
+  share2 #_ #emp_inames b;
+  assert (pts_to b #one_half A);
+  assert (pts_to b #one_half A ** emp);
+
   rewrite emp
        as `@(if false then pts_to y 42 else emp);
-  assert (pts_to b #(half_perm full_perm) false ** `@(if false then pts_to y 42 else emp));
-  assert (exists_ (fun (bb:bool) ->
-             pts_to b #(half_perm full_perm) bb ** (if bb then pts_to y 42 else emp)));
-  let i = mk_inv (exists_ (fun (bb:bool) ->
-             pts_to b #(half_perm full_perm) bb ** (if bb then pts_to y 42 else emp)));
+  assert (pts_to b #one_half A ** `@(if A = B then pts_to y 42 else emp));
+
+  assert (exists_ (fun (bb:abc) ->
+             pts_to b #one_half bb ** (if bb = B then pts_to y 42 else emp)));
+
+  fold invp b y;
+  let i = mk_inv (invp b y);
+
+  let pp =
+    make_promise
+      (pts_to_b_or_c b)
+      (pts_to y 42)
+      emp
+      (fun () -> test_aux_with_inv2 b y i);
+
   y := 42;
-  make_promise
-    (pts_to b #(half_perm full_perm) true)
-    (pts_to y 42)
-    emp
-    (fun () -> with_inv
-                 #unit
-                 #(pts_to b true ** emp)
-                 #(fun () -> pts_to b false ** pts_to y 42)
-                 #(exists_ (fun (bb:bool) -> pts_to b #(half_perm full_perm) bb ** (if bb then pts_to y 42 else emp)))
-               i
-               (fun () -> test_aux b y)
-  );
-  admit()
-//   admit()
+
+  // Set b:=B, keeping the invariant.
+  // FIXME: shouldn't have to talk about promise and y?
+  with_invariants i ensures
+     promise (pts_to_b_or_c b) (pts_to y 42)
+     //** pts_to y 42
+     ** pts_to b #one_half B
+  {
+    unfold invp b y;
+    assert (exists bb. pts_to b #one_half bb ** `@(if bb = B then pts_to y 42 else emp));
+    with ba.
+      assert (pts_to b #one_half ba ** `@(if ba = B then pts_to y 42 else emp));
+
+    assert (pts_to b #one_half A);
+
+    // Automate?
+    pts_to_injective_eq #abc
+          #one_half #one_half
+          #A #ba
+          b;
+
+    assert (pure (ba == A));
+
+    gather2 #_ #emp_inames b;
+    b := B;
+    share2 #_ #emp_inames b;
+
+    assert (pts_to b #one_half B ** `@(if B = B then pts_to y 42 else emp));
+    intro_exists (fun (bb:abc) -> pts_to b #one_half bb ** (if bb = B then pts_to y 42 else emp))
+      B;
+    fold (invp b y);
+    assert (invp b y);
+
+    // Pretty hard to find out to do this.
+    rewrite (`@(if ba = B then pts_to y 42 else emp))
+         as emp;
+
+    assert (pts_to b #one_half B);
+
+    ()
+  };
+
+  assert (pts_to b #one_half B);
+  fold (pts_to_b_or_c b);
+  assert (pts_to_b_or_c b);
+  redeem_promise (pts_to_b_or_c b) (pts_to y 42);
+
+  assert (pts_to y 42);
+  drop_ (pts_to_b_or_c b);
+
+  1234 
 }
 ```
